\subsection{}
For $ E_1 $:
\begin{equation*}
    n_x = 1 \textrm{, } n_y = 1 \textrm{, } n_z  = 1
\end{equation*}

For $ E_2 $:
\begin{align*}
    & n_x = 2 \textrm{, } n_y = 1 \textrm{, } n_z  = 1\\
    & n_x = 1 \textrm{, } n_y = 2 \textrm{, } n_z  = 1\\
    & n_x = 1 \textrm{, } n_y = 1 \textrm{, } n_z  = 2
\end{align*}

\subsection{}
Given:
\begin{equation*}
    \Delta E = E_2 - E_1 = hf = \frac{ch}{\lambda}
\end{equation*}
Then:
\begin{align*}
    \lambda & = \frac{ch}{E_2 - E_1}\\
    & = \frac{\SI{3e8}{\metre\second\tothe{-1}} \times \SI{6.63e-34}{\joule\second}}{\del{\del{2^2 + 1^2 + 1^2} - \del{1^2 + 1^2 + 1^2}} \times \SI{7.79}{\electronvolt} \times \SI{1.6e-19}{\joule\electronvolt\tothe{-1}}}\\
    & = \SI{5.32e-8}{\metre} \textrm{ (to 3 s.f.)}
\end{align*}
