\subsection{}
The coefficient rule for normalisation:
\begin{equation*}
    \sum_n \abs{a_n}^2 = 1
\end{equation*}
when applied to $ \Psi \del{x, 0} $ gives:
\begin{align*}
    \abs{C}^2 + \abs{-\operatorname{i}}^2 \abs{C}^2 + \abs{2C}^2 & = 1\\
    \abs{C}^2 + \abs{C}^2 + 4 \abs{C}^2 & = 1\\
    6 \abs{C}^2 & = 1\\
    \abs{C}^2 & = \frac{1}{6}\\
    P_{E_0} & = \abs{C}^2 = \frac{1}{6}\\
    P_{E_1} & = \abs{-\operatorname{i}}^2 \abs{C}^2 = \frac{1}{6}\\
    P_{E_3} & = \abs{2C}^2 = \frac{4}{6} = \frac{2}{3}
\end{align*}

\subsection{}
\begin{align*}
    \expectationvalue{E} & = \abs{C}^2 E_0 + \abs{C}^2 E_1 + \abs{2C}^2 E_3\\
    & = \frac{1}{6} \del{\frac{\hbar \omega}{2}} + \frac{1}{6} \del{\frac{3 \hbar \omega}{2}} + \frac{4}{6} \del{\frac{7 \hbar \omega}{2}}\\
    & = \frac{32 \hbar \omega}{12} = \frac{8 \hbar \omega}{3}
\end{align*}