\subsection{}

By definition,

\begin{align*}
  [\hat{p}_x, \hat{x}^n] = \hat{p}_x \hat{x}^n - \hat{x}^n \hat{p}_x
\end{align*}

We allow this operator to act on an arbitrary function $f(x)$:

\begin{align*}
  [\hat{p}_x, \hat{x}^n] f(x) = \hat{p}_x \hat{x}^n f(x) - \hat{x}^n \hat{p}_x f(x)
\end{align*}

where $\hat{p}_x = -i\hbar \frac{\partial}{\partial{x}}$, and $\hat{x}^n = x^n$.

\begin{align*}
  \hat{p}_x \hat{x}^n f(x) - \hat{x}^n \hat{p}_x f(x) =
    -i\hbar \frac{\partial}{\partial{x}} \big( x^n f(x) \big) - x^n (-i\hbar) \frac{\partial}{\partial{x}} f(x) = \\
    -i\hbar \, n \, x^{n-1} f(x) - i\hbar \, x^n \, \frac{\partial}{\partial{x}} f(x) + i\hbar \, x^n \, \frac{\partial}{\partial{x}} f(x)
\end{align*}

The final two terms trivially cancel out, thus

\begin{align*}
  [\hat{p}_x, \hat{x}^n] f(x) = -i\hbar \, n \, x^{n-1} f(x) \implies [\hat{p}_x, \hat{x}^n] = -i\hbar \, n \, x^{n-1}.
\end{align*}

\subsection{}

Generalized Ehrenfest theorem:

\begin{align*}
  \frac{\dif{\langle \textrm{A} \rangle}}{\dif{t}} = \frac{1}{i\hbar} \langle \big[ \hat{\textrm{A}}, \hat{\textrm{H}} \big] \rangle
\end{align*}

where $\hat{\textrm{H}}$ is the Hamiltonian operator of the system, and $\hat{\textrm{A}}$ is the observable in question. In our case:

\begin{align*}
  \frac{\dif{\langle p_x \rangle}}{\dif{t}} = \frac{1}{i\hbar} \langle \big[ \hat{\textrm{p}}_x, \hat{\textrm{H}} \big] \rangle
\end{align*}

Evaluating the commutator:

\begin{align*}
  \big[ \hat{\textrm{p}}_x, \hat{\textrm{H}} \big] &= \big[ \hat{\textrm{p}}_x, \frac{\hat{\textrm{p}}_{x}^2}{2m} + \frac{1}{2} C \hat{\textrm{x}}^4 \big] \\
    &= \big[ \hat{\textrm{p}}_x, \frac{\hat{\textrm{p}}_{x}^2}{2m} \big] + \big[ \hat{\textrm{p}}_x, \frac{1}{2} C \hat{\textrm{x}}^4 \big] \\
    &= \frac{1}{2m} \big[ \hat{\textrm{p}}_x, \hat{\textrm{p}}_{x}^2 \big] + \frac{C}{2} \big[ \hat{\textrm{p}}_x, \hat{\textrm{x}}^4 \big] \\
    &= 4 (-i\hbar) \frac{C}{2} x^3
\end{align*}

because $[\hat{\textrm{p}}_x, \hat{\textrm{p}}_{x}^2]$ trivially commutes. Thus,

\begin{align*}
  \frac{\dif{\langle p_x \rangle}}{\dif{t}} &= \frac{1}{i\hbar} \langle -2 i\hbar C x^3 \rangle \\
    &= -2 C \langle x^3 \rangle
\end{align*}
